theories/logatom/conditional_increment/spec.v
@@ -1,0 +1,50 @@
+From stdpp Require Import namespaces.
+From iris.heap_lang Require Export lifting notation.
+From iris.program_logic Require Export atomic.
+Set Default Proof Using "Type".
+
+(** A general logically atomic interface for conditional increment. *)
+Record atomic_cinc {Σ} `{!heapG Σ} := AtomicCinc {
+  (* -- operations -- *)
+  new_counter : val;
+  cinc : val;
+  set_flag : val;
+  get : val;
+  (* -- other data -- *)
+  name : Type;
+  name_eqdec : EqDecision name;
+  name_countable : Countable name;
+  (* -- predicates -- *)
+  is_counter (N : namespace) (γs : name) (v : val) : iProp Σ;
+  counter_content (γs : name) (flag : bool) (c : Z) : iProp Σ;
+  (* -- predicate properties -- *)
+  is_counter_persistent N γs v : Persistent (is_counter N γs v);
+  counter_content_timeless γs f c : Timeless (counter_content γs f c);
+  counter_content_exclusive γs f1 c1 f2 c2 :
+    counter_content γs f1 c1 -∗ counter_content γs f2 c2 -∗ False;
+  (* -- operation specs -- *)
+  new_counter_spec N :
+    {{{ True }}}
+        new_counter #()
+    {{{ ctr γs, RET ctr ; is_counter N γs ctr ∗ counter_content γs true 0 }}};
+  cinc_spec N γs v :
+    is_counter N γs v -∗
+    <<< ∀ (b : bool) (n : Z), counter_content γs b n >>>
+        cinc v @⊤∖↑N
+    <<< counter_content γs b (if b then n + 1 else n), RET #() >>>;
+  set_flag_spec N γs v (new_b: bool) :
+    is_counter N γs v -∗
+    <<< ∀ (b : bool) (n : Z), counter_content γs b n >>>
+        set_flag v #new_b @⊤∖↑N
+    <<< counter_content γs new_b n, RET #() >>>;
+  get_spec N γs v:
+    is_counter N γs v -∗
+    <<< ∀ (b : bool) (n : Z), counter_content γs b n >>>
+        get v @⊤∖↑N
+    <<< counter_content γs b n, RET #n >>>;
+}.
+Arguments atomic_cinc _ {_}.
+
+Existing Instances
+  is_counter_persistent counter_content_timeless
+  name_countable name_eqdec.
